proof/infoflow/AARCH64/ArchDecode_IF.thy
@@ -46,19 +46,21 @@ lemma arch_decode_irq_control_invocation_rev[Decode_IF_assms]:
      (arch_decode_irq_control_invocation label args slot caps)"
   unfolding arch_decode_irq_control_invocation_def arch_check_irq_def
   apply (wp ensure_empty_rev lookup_slot_for_cnode_op_rev
-            is_irq_active_rev whenE_inv
+            is_irq_active_rev whenE_inv range_check_ev
          | wp (once) hoare_drop_imps
-         | simp add: Let_def)+
+         | simp add: Let_def unlessE_def split del: if_split)+
   apply safe
-       apply simp+
-    apply (blast intro: aag_Control_into_owns_irq )
+           apply simp+
+      apply (blast intro: aag_Control_into_owns_irq)
+     apply (drule_tac x="caps ! 0" in bspec)
+      apply (fastforce intro: bang_0_in_set)
+     apply (drule (1) is_cnode_into_is_subject; blast dest: prop_of_obj_ref_of_cnode_cap)
+    apply (fastforce dest: is_cnode_into_is_subject intro: bang_0_in_set)
    apply (drule_tac x="caps ! 0" in bspec)
     apply (fastforce intro: bang_0_in_set)
    apply (drule (1) is_cnode_into_is_subject; blast dest: prop_of_obj_ref_of_cnode_cap)
   apply (fastforce dest: is_cnode_into_is_subject intro: bang_0_in_set)
   done
-
-requalify_facts check_valid_ipc_buffer_inv
 
 end
 
@@ -172,6 +174,16 @@ lemma decode_asid_control_invocation_reads_respects_f:
   apply fastforce
   done
 
+(* FIXME AARCH64 IF: proof cleanup *)
+
+lemma
+  notes reads_respects_f_inv' = reads_respects_f_inv[where st=st]
+  notes whenE_wps[wp_split del]
+  shows reads_respects_f_check_vspace_root[wp]:
+  "reads_respects_f aag l \<top> (check_vspace_root cap arg)"
+  unfolding check_vspace_root_def
+  by (rule equiv_valid_guard_imp, wpsimp+)
+
 lemma decode_frame_invocation_reads_respects_f:
   notes reads_respects_f_inv' = reads_respects_f_inv[where st=st]
   notes whenE_wps[wp_split del]
@@ -179,15 +191,69 @@ lemma decode_frame_invocation_reads_respects_f:
     "reads_respects_f aag l
        (silc_inv aag st and invs and pas_refined aag and cte_wp_at ((=) (cap.ArchObjectCap cap)) slot
                         and (\<lambda>s. \<forall>(cap, slot) \<in> set excaps. cte_wp_at ((=) cap) slot s)
-                        and K (cap = FrameCap p R sz dev m)
+                        and valid_arch_cap cap and K (cap = FrameCap p R sz dev m)
                         and K (\<forall>(cap, slot) \<in> {(cap.ArchObjectCap cap, slot)} \<union> set excaps.
                                  aag_cap_auth aag (pasObjectAbs aag (fst slot)) cap \<and>
                                  is_subject aag (fst slot) \<and>
                                  (\<forall>v \<in> cap_asid' cap. is_subject_asid aag v)))
         (decode_frame_invocation label args slot cap excaps)"
   unfolding decode_frame_invocation_def decode_fr_inv_map_def
-            check_slot_def check_vp_alignment_def gets_the_def
+            check_vp_alignment_def gets_the_def
+ apply (rule gen_asm_ev)+
   supply gets_the_ev[wp del]
+  apply (case_tac "invocation_type label = ArchInvocationLabel ARMPageMap")
+   apply (clarsimp split del: if_split)
+  apply (rule equiv_valid_guard_imp)
+    apply ((wp gets_ev' check_vp_wpR  reads_respects_f_inv'[OF get_asid_pool_rev]
+               reads_respects_f_inv'[OF ensure_empty_rev]
+               reads_respects_f_inv'[OF get_pte_rev]
+               reads_respects_f_inv'[OF lookup_slot_for_cnode_op_rev]
+               reads_respects_f_inv'[OF ensure_no_children_rev]
+               reads_respects_f_inv'[OF lookup_error_on_failure_rev]
+               find_vspace_for_asid_reads_respects
+               is_final_cap_reads_respects
+               select_ext_ev_bind_lift
+               select_ext_ev_bind_lift[simplified]
+            | wpc
+            | simp add: Let_def unlessE_whenE
+            | wp (once) whenE_throwError_wp)+)[1]
+   apply clarsimp
+   apply (drule_tac x="excaps ! 0" in bspec, fastforce intro: bang_0_in_set)+
+   apply clarsimp
+   apply (rule conjI)
+    apply (fastforce dest: cte_wp_valid_cap simp: valid_cap_def wellformed_mapdata_def)
+   apply clarsimp
+   apply (case_tac "m = None \<and> \<not> user_vtop < args ! 0 + mask (pageBitsForSize sz) \<or> (m = Some (asid, args ! 0))")
+    prefer 2
+    apply clarsimp
+   apply (prop_tac "\<not> user_vtop < args ! 0 + mask (pageBitsForSize sz) \<longrightarrow> args ! 0 \<in> user_region")
+    apply (clarsimp simp: user_region_def not_le)
+    apply (rule user_vtop_leq_canonical_user)
+    apply (simp add: vmsz_aligned_def not_less)
+    apply (drule is_aligned_no_overflow_mask)
+    apply simp
+   apply (prop_tac "args ! 0 \<in> user_region")
+    apply (fastforce simp: valid_arch_cap_def wellformed_mapdata_def)
+   apply (subgoal_tac "(\<forall>t. reads_equiv_f aag s t \<and> affects_equiv aag l s t \<longrightarrow>
+                    pt_lookup_slot pt (args ! 0) (ptes_of s) = pt_lookup_slot pt (args ! 0) (ptes_of t))")
+    apply clarsimp
+   apply (clarsimp simp: reads_equiv_f_def)
+   apply (frule vspace_for_asid_vs_lookup)
+   apply (frule_tac pt=pt and level=max_pt_level and bot_level=0 in pt_walk_reads_equiv,
+          (fastforce dest: aag_has_Control_iff_owns
+                     elim: vs_lookup_table_vref_independent
+                     simp: aag_cap_auth_def cap_auth_conferred_def arch_cap_auth_conferred_def
+                           pt_lookup_slot_def pt_lookup_slot_from_level_def obind_def
+                    split: option.splits)+)[1]
+  apply (case_tac "invocation_type label = ArchInvocationLabel ARMPageUnmap")
+   apply wpsimp
+  apply (case_tac "invocation_type label = ArchInvocationLabel ARMPageGetAddress")
+   apply wpsimp
+  apply (case_tac "isPageFlushLabel (invocation_type label)")
+   prefer 2
+   apply wpsimp
+  apply (clarsimp split del: if_split)
+  apply (unfold decode_fr_inv_flush_def)
   apply (rule equiv_valid_guard_imp)
    apply ((wp gets_ev' check_vp_wpR  reads_respects_f_inv'[OF get_asid_pool_rev]
               reads_respects_f_inv'[OF ensure_empty_rev]
@@ -203,36 +269,25 @@ lemma decode_frame_invocation_reads_respects_f:
            | simp add: Let_def unlessE_whenE
            | wp (once) whenE_throwError_wp)+)[1]
   apply clarsimp
-  apply (drule_tac x="excaps ! 0" in bspec, fastforce intro: bang_0_in_set)+
-  apply (intro conjI; clarsimp)
-   apply (fastforce dest: cte_wp_valid_cap simp: valid_cap_def wellformed_mapdata_def)
-  apply (prop_tac "args ! 0 \<in> user_region")
-   apply (drule not_le_imp_less)
-   apply (frule order.strict_implies_order[where b=user_vtop])
-   apply (drule order.strict_trans[OF _ user_vtop_pptr_base])
-   apply (drule canonical_below_pptr_base_user)
-    apply (erule below_user_vtop_canonical)
-   apply (clarsimp simp: user_region_def)
-   apply (drule is_aligned_no_overflow_mask)
-   apply (erule (1) dual_order.trans)
-  apply (rule conjI; clarsimp)
-   apply (clarsimp simp: reads_equiv_f_def)
-   apply (frule vspace_for_asid_vs_lookup)
-   apply (frule_tac pt=xa and level=max_pt_level and bot_level=0 in pt_walk_reads_equiv,
-          (fastforce dest: aag_has_Control_iff_owns
-                     elim: vs_lookup_table_vref_independent
-                     simp: aag_cap_auth_def cap_auth_conferred_def arch_cap_auth_conferred_def
-                           pt_lookup_slot_def pt_lookup_slot_from_level_def obind_def
-                    split: option.splits)+)[1]
-  apply (subgoal_tac "is_subject aag (table_base bb)", clarsimp)
-  apply (clarsimp simp: pt_lookup_slot_def pt_lookup_slot_from_level_def vspace_for_asid_def)
-  apply (frule pt_walk_is_aligned)
-   apply (erule (1) vspace_for_pool_is_aligned[OF _ _ user_region0]; clarsimp)
-  apply clarsimp
-  apply (erule_tac asid=a in pt_walk_is_subject[rotated 4]; clarsimp?)
-   apply (clarsimp simp: vs_lookup_table_def in_omonad)
-  apply (fastforce intro: vspace_for_asid_is_subject simp: vspace_for_asid_def in_omonad)
+  apply (clarsimp simp: valid_arch_cap_def wellformed_mapdata_def)
   done
+
+lemma helper:
+  "reads_respects_f aag l (pt_at pt_t (table_base pt_t p) and K (is_subject aag (table_base pt_t p)))
+            (do m <- gets (swp ptes_of pt_t);
+                        assert_opt (m p)
+                     od)"
+  apply (auto simp: equiv_valid_def2 equiv_valid_2_def bind_def gets_def assert_opt_def fail_def
+  get_def return_def split: option.splits)
+  apply (drule ptes_of_reads_equiv)
+   apply (fastforce simp: reads_equiv_f_def)
+  apply clarsimp
+  done
+
+definition foldme where
+  "foldme level slot \<equiv> liftE $ do m <- gets (swp ptes_of (level_type level));
+                                               assert_opt (m slot)
+                                            od"
 
 lemma decode_page_table_invocation_reads_respects_f:
   notes reads_respects_f_inv' = reads_respects_f_inv[where st=st]
@@ -241,15 +296,16 @@ lemma decode_page_table_invocation_reads_respects_f:
     "reads_respects_f aag l
        (silc_inv aag st and invs and pas_refined aag and cte_wp_at ((=) (cap.ArchObjectCap cap)) slot
                         and (\<lambda>s. \<forall>(cap, slot) \<in> set excaps. cte_wp_at ((=) cap) slot s)
-                        and K (cap = PageTableCap p m)
+                        and valid_arch_cap cap and K (cap = PageTableCap p pt_t m)
                         and K (\<forall>(cap, slot) \<in> {(cap.ArchObjectCap cap, slot)} \<union> set excaps.
                                  aag_cap_auth aag (pasObjectAbs aag (fst slot)) cap \<and>
                                  is_subject aag (fst slot) \<and>
                                  (\<forall>v \<in> cap_asid' cap. is_subject_asid aag v)))
         (decode_page_table_invocation label args slot cap excaps)"
-  unfolding decode_page_table_invocation_def decode_pt_inv_map_def gets_the_def
+  unfolding decode_page_table_invocation_def decode_pt_inv_map_def gets_the_def gets_map_def
   supply gets_the_ev[wp del]
   apply (rule equiv_valid_guard_imp)
+   apply (fold foldme_def)
    apply ((wp gets_ev' check_vp_wpR reads_respects_f_inv'[OF get_asid_pool_rev]
               reads_respects_f_inv'[OF ensure_empty_rev]
               reads_respects_f_inv'[OF get_pte_rev]
@@ -263,43 +319,97 @@ lemma decode_page_table_invocation_reads_respects_f:
            | simp add: Let_def unlessE_whenE if_fun_split
            | wpc
            | wp (once) whenE_throwError_wp hoare_drop_imps)+)[1]
+  apply (unfold foldme_def)
+                    apply simp
+                    apply (wp (once))
+                    apply (rule helper)
+   apply ((wp gets_ev' check_vp_wpR reads_respects_f_inv'[OF get_asid_pool_rev]
+              reads_respects_f_inv'[OF ensure_empty_rev]
+              reads_respects_f_inv'[OF get_pte_rev]
+              reads_respects_f_inv'[OF lookup_slot_for_cnode_op_rev]
+              reads_respects_f_inv'[OF ensure_no_children_rev]
+              reads_respects_f_inv'[OF lookup_error_on_failure_rev]
+              find_vspace_for_asid_reads_respects
+              is_final_cap_reads_respects
+              select_ext_ev_bind_lift
+              select_ext_ev_bind_lift[simplified]
+           | simp add: Let_def unlessE_whenE if_fun_split
+           | wpc
+           | wp (once) whenE_throwError_wp hoare_drop_imps)+)
   apply clarsimp
   apply (rule conjI; clarsimp)
    apply (drule_tac x="excaps ! 0" in bspec, fastforce intro: bang_0_in_set)+
    apply (prop_tac "args ! 0 \<in> user_region")
-    apply (drule not_le_imp_less)
-    apply (frule order.strict_implies_order[where b=user_vtop])
-    apply (drule order.strict_trans[OF _ user_vtop_pptr_base])
-    apply (drule canonical_below_pptr_base_user)
-     apply (erule below_user_vtop_canonical)
-    apply (clarsimp simp: user_region_def)
-   apply clarsimp
-   apply (intro conjI impI allI; clarsimp)
+    apply (clarsimp simp: user_region_def not_le)
+    apply (rule user_vtop_leq_canonical_user)
+    apply (simp add: vmsz_aligned_def not_less)
+   apply (clarsimp cong: conj_cong imp_cong)
+   apply (rule conjI)
      apply (fastforce dest: cte_wp_valid_cap simp: valid_cap_def wellformed_mapdata_def)
+  apply (intro impI)
+   apply (rule context_conjI; clarsimp)
     apply (clarsimp simp: reads_equiv_f_def)
     apply (frule vspace_for_asid_vs_lookup)
-    apply (frule_tac pt=xa and level=max_pt_level and bot_level=0 in pt_walk_reads_equiv,
+    apply (frule_tac pt=pt and level=max_pt_level and bot_level=0 in pt_walk_reads_equiv,
            (fastforce dest: aag_has_Control_iff_owns
                       elim: vs_lookup_table_vref_independent
                       simp: aag_cap_auth_def cap_auth_conferred_def arch_cap_auth_conferred_def
                             pt_lookup_slot_def pt_lookup_slot_from_level_def obind_def
                      split: option.splits)+)[1]
-   apply (clarsimp simp: pt_lookup_slot_def pt_lookup_slot_from_level_def vspace_for_asid_def)
-   apply (frule pt_walk_is_aligned)
-    apply (erule (1) vspace_for_pool_is_aligned[OF _ _ user_region0]; clarsimp)
-   apply clarsimp
-   apply (erule_tac asid=a in pt_walk_is_subject[rotated 4]; clarsimp?)
-    apply (clarsimp simp: vs_lookup_table_def in_omonad)
-   apply (fastforce intro: vspace_for_asid_is_subject simp: vspace_for_asid_def in_omonad)
-  apply (rule conjI, fastforce elim!: is_subject_not_silc_inv)+
-  apply (clarsimp simp: reads_equiv_f_def)
-  apply (erule reads_equivE)
-  apply (clarsimp simp: equiv_asids_def equiv_asid_def)
-  apply (erule_tac x=a in allE)
-  apply (fastforce simp: vspace_for_asid_def pool_for_asid_def vspace_for_pool_def
-                         asid_pools_of_ko_at obj_at_def obind_def opt_map_def
-                  split: option.splits)
+
+   apply (rule conjI)
+    apply (frule (3) pt_lookup_slot_pte_at)
+    apply (clarsimp simp: pte_at_def2)
+   apply (frule vspace_for_asid_is_subject, fastforce+)
+   apply (clarsimp simp: pt_lookup_slot_def)
+   apply (erule pt_lookup_slot_from_level_is_subject)
+          apply fastforce+
+      apply (fastforce dest: vspace_for_asid_vs_lookup vs_lookup_table_vref_independent)
+     apply clarsimp+
+  apply (intro conjI)
+     apply fastforce
+     apply fastforce
+     apply fastforce
+  apply (fastforce dest: silc_inv_not_subject)
   done
+
+lemma decode_vspace_invocation_reads_respects_f:
+  notes reads_respects_f_inv' = reads_respects_f_inv[where st=st]
+  notes whenE_wps[wp_split del]
+  shows
+    "reads_respects_f aag l
+       (silc_inv aag st and invs and pas_refined aag and cte_wp_at ((=) (cap.ArchObjectCap cap)) slot
+                        and (\<lambda>s. \<forall>(cap, slot) \<in> set excaps. cte_wp_at ((=) cap) slot s)
+                        and valid_arch_cap cap
+                        and K (\<forall>(cap, slot) \<in> {(cap.ArchObjectCap cap, slot)} \<union> set excaps.
+                                 aag_cap_auth aag (pasObjectAbs aag (fst slot)) cap \<and>
+                                 is_subject aag (fst slot) \<and>
+                                 (\<forall>v \<in> cap_asid' cap. is_subject_asid aag v)))
+        (decode_vspace_invocation label args slot cap excaps)"
+  unfolding decode_vspace_invocation_def decode_vs_inv_flush_def
+  sorry
+
+lemma decode_vcpu_invocation_reads_respects_f:
+  notes reads_respects_f_inv' = reads_respects_f_inv[where st=st]
+  notes whenE_wps[wp_split del]
+  shows
+    "reads_respects_f aag l
+       (silc_inv aag st and invs and pas_refined aag and cte_wp_at ((=) (cap.ArchObjectCap cap)) slot
+                        and (\<lambda>s. \<forall>(cap, slot) \<in> set excaps. cte_wp_at ((=) cap) slot s)
+                        and valid_arch_cap cap
+                        and K (\<forall>(cap, slot) \<in> {(cap.ArchObjectCap cap, slot)} \<union> set excaps.
+                                 aag_cap_auth aag (pasObjectAbs aag (fst slot)) cap \<and>
+                                 is_subject aag (fst slot) \<and>
+                                 (\<forall>v \<in> cap_asid' cap. is_subject_asid aag v)))
+        (decode_vcpu_invocation label args cap excaps)"
+  unfolding decode_vcpu_invocation_def
+  sorry
+
+lemma decode_sgi_signal_invocation_reads_respects_f[wp]:
+  "reads_respects_f aag l \<top>
+        (decode_sgi_signal_invocation (SGISignalCap x61 x62))"
+  unfolding decode_sgi_signal_invocation_def
+  by wpsimp
 
 lemma arch_decode_invocation_reads_respects_f[Decode_IF_assms]:
   notes reads_respects_f_inv' = reads_respects_f_inv[where st=st]
@@ -314,11 +424,15 @@ lemma arch_decode_invocation_reads_respects_f[Decode_IF_assms]:
                                  (\<forall>v \<in> cap_asid' cap. is_subject_asid aag v)))
         (arch_decode_invocation label args cap_index slot cap excaps)"
   unfolding arch_decode_invocation_def
-  apply (cases cap; rule equiv_valid_guard_imp)
+  apply (cases cap; clarsimp; rule equiv_valid_guard_imp)
   by (wpsimp wp: decode_asid_pool_invocation_reads_respects_f
                  decode_asid_control_invocation_reads_respects_f
                  decode_frame_invocation_reads_respects_f
-                 decode_page_table_invocation_reads_respects_f | fastforce)+
+                 decode_vspace_invocation_reads_respects_f
+                 decode_vcpu_invocation_reads_respects_f
+                 decode_page_table_invocation_reads_respects_f
+      | fastforce dest: caps_of_state_valid cte_wp_at_caps_of_state'
+                  simp: valid_cap_def valid_arch_cap_def)+
 
 end
 
