proof/infoflow/AARCH64/ArchFinalCaps.thy
@@ -46,14 +46,41 @@ lemma set_asid_pool_silc_inv[wp]:
   apply (fastforce elim: cte_wp_atE intro: cte_wp_at_cteI cte_wp_at_tcbI)
   done
 
-crunch arch_finalise_cap, prepare_thread_delete, init_arch_objects
+lemma set_vcpu_silc_inv:
+  "\<lbrace>silc_inv aag st\<rbrace>
+   set_vcpu ptr vcpu
+   \<lbrace>\<lambda>_. silc_inv aag st\<rbrace>"
+  unfolding set_vcpu_def
+  apply (rule silc_inv_pres)
+    apply (wpsimp wp: set_object_wp_strong get_object_wp simp: obj_at_def)
+    apply (drule (1) silc_inv_cnode_only)
+    apply (fastforce simp: silc_inv_def obj_at_def is_cap_table_def split: kernel_object.splits)
+   apply (wpsimp wp: set_object_wp get_object_wp)
+  apply (wpsimp wp: set_object_wp_strong get_object_wp simp: obj_at_def)
+  apply (case_tac "ptr = fst (a,b)")
+   apply (fastforce elim: cte_wp_atE simp: obj_at_def)
+  apply (fastforce elim: cte_wp_atE intro: cte_wp_at_cteI cte_wp_at_tcbI)
+  done
+
+crunch vcpu_switch
+  for silc_inv[wp]: "silc_inv aag st"
+  (wp: mapM_x_wp_inv mapM_wp_inv)
+
+crunch associate_vcpu_tcb
+  for silc_inv[wp]: "silc_inv aag st"
+  (wp: crunch_wps simp: arch_thread_set_is_thread_set)
+
+crunch arch_finalise_cap, prepare_thread_delete
   for silc_inv[FinalCaps_assms, wp]: "silc_inv aag st"
   (wp: crunch_wps modify_wp simp: crunch_simps ignore: set_object)
 
-crunch handle_reserved_irq, handle_vm_fault, handle_hypervisor_fault, handle_arch_fault_reply,
-         arch_invoke_irq_handler, arch_mask_irq_signal,
-         arch_post_cap_deletion, arch_post_modify_registers,
-         arch_activate_idle_thread, arch_switch_to_idle_thread, arch_switch_to_thread
+crunch init_arch_objects
+  for silc_inv[FinalCaps_assms, wp]: "silc_inv aag st"
+  (wp: crunch_wps modify_wp simp: crunch_simps ignore: set_object)
+
+crunch handle_vm_fault, handle_arch_fault_reply, arch_invoke_irq_handler, arch_mask_irq_signal,
+       arch_post_cap_deletion, arch_post_modify_registers, arch_activate_idle_thread,
+       arch_switch_to_idle_thread, arch_switch_to_thread
   for silc_inv[FinalCaps_assms, wp]: "silc_inv aag st"
 
 lemma arch_derive_cap_silc[FinalCaps_assms]:
@@ -69,7 +96,6 @@ lemma arch_derive_cap_silc[FinalCaps_assms]:
 declare init_arch_objects_cte_wp_at[FinalCaps_assms]
 declare handle_vm_fault_cur_thread[FinalCaps_assms]
 declare finalise_cap_makes_halted[FinalCaps_assms]
-declare init_arch_objects_inv[FinalCaps_assms]
 
 end
 
@@ -112,12 +138,15 @@ lemma perform_page_table_invocation_silc_inv_get_cap_helper:
 lemmas perform_page_table_invocation_silc_inv_get_cap_helper' =
   perform_page_table_invocation_silc_inv_get_cap_helper[simplified o_def fun_app_def]
 
+crunch store_pte
+  for silc_inv[FinalCaps_assms, wp]: "silc_inv aag st"
+
 lemma mapM_x_swp_store_pte_silc_inv[wp]:
-  "mapM_x (swp store_pte A) slots \<lbrace>silc_inv aag st\<rbrace>"
+  "mapM_x (swp (store_pte pt_t) A) slots \<lbrace>silc_inv aag st\<rbrace>"
   by (wp mapM_x_wp[OF _ subset_refl] | simp add: swp_def)+
 
 lemma is_arch_eq_pt_is_pt_or_frame_cap:
-  "cte_wp_at ((=) (ArchObjectCap (PageTableCap xa xb))) slot s
+  "cte_wp_at ((=) (ArchObjectCap (PageTableCap pt_t xa xb))) slot s
    \<Longrightarrow> cte_wp_at (\<lambda>a. is_pt_cap a \<or> is_frame_cap a) slot s"
   apply (erule cte_wp_at_weakenE)
   by (clarsimp simp: is_frame_cap_def is_pt_cap_def)
@@ -127,6 +156,9 @@ lemma is_arch_eq_pg_is_pt_or_pg_cap:
    \<Longrightarrow> cte_wp_at (\<lambda>a. is_pt_cap a \<or> is_frame_cap a) slot s"
   apply (erule cte_wp_at_weakenE)
   by (clarsimp simp: is_frame_cap_def is_pt_cap_def)
+
+crunch unmap_page_table
+  for silc_inv[FinalCaps_assms, wp]: "silc_inv aag st"
 
 lemma perform_page_table_invocation_silc_inv:
   "\<lbrace>silc_inv aag st and valid_pti blah and K (authorised_page_table_inv aag blah)\<rbrace>
@@ -151,6 +183,13 @@ lemma perform_page_table_invocation_silc_inv:
   apply fastforce
   done
 
+crunch invalidate_tlb_by_asid_va, perform_flush
+  for silc_inv[FinalCaps_assms, wp]: "silc_inv aag st"
+
+crunch unmap_page
+  for silc_inv[FinalCaps_assms, wp]: "silc_inv aag st"
+  (simp: crunch_simps)
+
 lemma perform_page_invocation_silc_inv:
   "\<lbrace>silc_inv aag st and valid_page_inv blah and authorised_page_inv aag blah\<rbrace>
    perform_page_invocation blah
@@ -167,10 +206,15 @@ lemma perform_page_invocation_silc_inv:
   apply (clarsimp simp: valid_page_inv_def authorised_page_inv_def
                   split: page_invocation.splits)
    apply (intro allI impI conjI)
-    apply (drule_tac slot="(ab,bc)" in overlapping_slots_have_labelled_overlapping_caps[rotated])
-      apply (fastforce)
+      apply (drule_tac slot="(ac,bb)" in overlapping_slots_have_labelled_overlapping_caps[rotated])
+        apply (fastforce)+
+       apply (fastforce elim: is_arch_update_overlaps[rotated] cte_wp_at_weakenE)
+      apply fastforce+
+     apply (fastforce simp: silc_inv_def)
+    apply (drule_tac slot="(ac,bb)" in overlapping_slots_have_labelled_overlapping_caps[rotated])
+      apply (fastforce)+
      apply (fastforce elim: is_arch_update_overlaps[rotated] cte_wp_at_weakenE)
-    apply fastforce
+    apply fastforce+
    apply (fastforce simp: silc_inv_def)
   apply (fastforce dest: is_arch_eq_pg_is_pt_or_pg_cap simp: silc_inv_def pred_disj_def)
   done
@@ -188,7 +232,7 @@ lemma perform_asid_control_invocation_silc_inv:
             set_cap_silc_inv get_cap_slots_holding_overlapping_caps[where st=st]
             delete_objects_silc_inv hoare_weak_lift_imp
          | wpc | simp )+
-  apply (clarsimp simp: authorised_asid_control_inv_def silc_inv_def valid_aci_def ptr_range_def page_bits_def)
+  apply (clarsimp simp: authorised_asid_control_inv_def silc_inv_def valid_aci_def ptr_range_def)
   apply (rule conjI)
    apply (clarsimp simp: range_cover_def obj_bits_api_def default_arch_object_def asid_bits_def pageBits_def)
    apply (rule of_nat_inverse)
@@ -206,10 +250,6 @@ lemma perform_asid_control_invocation_silc_inv:
 crunch store_asid_pool_entry, handle_spurious_irq
   for silc_inv[wp]: "silc_inv aag st"
 
-crunch copy_global_mappings
-  for silc_inv[wp]: "silc_inv aag st"
-  (wp: crunch_wps modify_wp simp: crunch_simps ignore: set_object)
-
 lemma perform_asid_pool_invocation_silc_inv:
   "\<lbrace>silc_inv aag st and K (authorised_asid_pool_inv aag blah)\<rbrace>
    perform_asid_pool_invocation blah
@@ -221,6 +261,9 @@ lemma perform_asid_pool_invocation_silc_inv:
                          slots_holding_overlapping_caps_def authorised_asid_pool_inv_def
                          is_ArchObjectCap_def is_PageTableCap_def update_map_data_def)+
   done
+
+crunch perform_vcpu_invocation, perform_vspace_invocation, perform_sgi_invocation
+  for silc_inv[wp]: "silc_inv aag st"
 
 declare handle_spurious_irq_silc_inv[wp, FinalCaps_assms]
 
@@ -234,8 +277,20 @@ lemma arch_perform_invocation_silc_inv[FinalCaps_assms]:
             perform_page_invocation_silc_inv
             perform_asid_control_invocation_silc_inv
             perform_asid_pool_invocation_silc_inv
+            perform_vcpu_invocation_silc_inv
          | wpc)+
   apply (clarsimp simp: authorised_arch_inv_def valid_arch_inv_def split: arch_invocation.splits)
+  done
+
+lemma new_irq_handler_caps_are_intra_label:
+  "\<lbrakk> cte_wp_at ((=) (IRQControlCap)) slot s; pas_refined aag s; is_subject aag (fst slot) \<rbrakk>
+     \<Longrightarrow> cap_points_to_label aag (IRQHandlerCap irq) (pasSubject aag)"
+  apply (clarsimp simp: cap_points_to_label_def)
+  apply (frule cap_cur_auth_caps_of_state[rotated])
+    apply assumption
+   apply (simp add: cte_wp_at_caps_of_state)
+  apply (clarsimp simp: aag_cap_auth_def cap_links_irq_def)
+  apply (blast intro: aag_Control_into_owns_irq)
   done
 
 lemma arch_invoke_irq_control_silc_inv[FinalCaps_assms]:
@@ -249,6 +304,7 @@ lemma arch_invoke_irq_control_silc_inv[FinalCaps_assms]:
   apply (wp cap_insert_silc_inv'' hoare_vcg_ex_lift slots_holding_overlapping_caps_lift
          | simp add: authorised_irq_ctl_inv_def arch_irq_control_inv_valid_def)+
   apply (fastforce dest: new_irq_handler_caps_are_intra_label)
+  apply (wpsimp wp: cap_insert_silc_inv'' simp: cap_points_to_label_def)
   done
 
 crunch set_priority, set_flags
@@ -256,7 +312,28 @@ crunch set_priority, set_flags
   (simp: tcb_cap_cases_def)
 
 crunch arch_prepare_set_domain, arch_prepare_next_domain, arch_post_set_flags
-  for inv[FinalCaps_assms,wp]: P
+  for silc_inv[FinalCaps_assms, wp]: "silc_inv aag st"
+  (wp: crunch_wps)
+
+
+lemma tcb_cap_cases_tcb_fault:
+  "\<forall>(getF, a, b)\<in>ran tcb_cap_cases.
+         getF (tcb_fault_update F tcb) = getF tcb"
+  by (rule ball_tcb_cap_casesI, simp+)
+
+lemma case_option_wp_returnOk:
+  assumes [wp]: "\<And>x. \<lbrace>P x\<rbrace> f x \<lbrace>\<lambda>_. Q\<rbrace>"
+  shows "\<lbrace>Q and (\<lambda>s. opt \<noteq> None \<longrightarrow> P (the opt) s)\<rbrace>
+         (case opt of None \<Rightarrow> returnOk rv | Some x \<Rightarrow> f x)
+         \<lbrace>\<lambda>_. Q\<rbrace>"
+  by (cases opt; wpsimp)
+
+lemma case_option_wp_return:
+  assumes [wp]: "\<And>x. \<lbrace>P x\<rbrace> f x \<lbrace>\<lambda>_. Q\<rbrace>"
+  shows "\<lbrace>Q and (\<lambda>s. opt \<noteq> None \<longrightarrow> P (the opt) s)\<rbrace>
+         (case opt of None \<Rightarrow> return rv | Some x \<Rightarrow> f x)
+         \<lbrace>\<lambda>_. Q\<rbrace>"
+  by (cases opt; wpsimp)
 
 lemma invoke_tcb_silc_inv[FinalCaps_assms]:
   notes hoare_weak_lift_imp [wp]
@@ -266,19 +343,21 @@ lemma invoke_tcb_silc_inv[FinalCaps_assms]:
          invoke_tcb tinv
          \<lbrace>\<lambda>_. silc_inv aag st\<rbrace>"
   apply (case_tac tinv)
-         apply ((wp restart_silc_inv hoare_vcg_if_lift suspend_silc_inv mapM_x_wp[OF _ subset_refl]
-                    hoare_weak_lift_imp
-                 | wpc
-                 | simp split del: if_split add: authorised_tcb_inv_def check_cap_at_def
-                 | clarsimp
-                 | strengthen invs_mdb
-                 | force intro: notE[rotated,OF idle_no_ex_cap,simplified])+)[3]
-      defer
-      apply ((wp suspend_silc_inv restart_silc_inv | simp add: authorised_tcb_inv_def | force)+)[2]
-    (* NotificationControl *)
-    apply (rename_tac option)
-    apply (case_tac option; (wp | simp)+)
-   (* SetTLSBase *)
+          apply ((wp restart_silc_inv hoare_vcg_if_lift suspend_silc_inv mapM_x_wp[OF _ subset_refl]
+                     hoare_weak_lift_imp
+                  | wpc
+                  | simp split del: if_split add: authorised_tcb_inv_def check_cap_at_def
+                  | clarsimp
+                  | strengthen invs_mdb
+                  | force intro: notE[rotated,OF idle_no_ex_cap,simplified])+)[3]
+       defer
+       apply ((wp suspend_silc_inv restart_silc_inv | simp add: authorised_tcb_inv_def | force)+)[2]
+     (* NotificationControl *)
+     apply (rename_tac option)
+     apply (case_tac option; (wp | simp)+)
+    (* SetTLSBase *)
+    apply (wpsimp split: option.splits)
+   (* SetFlags *)
    apply (wpsimp split: option.splits)
   (* just ThreadControl left *)
   apply (simp add: split_def cong: option.case_cong)
@@ -286,7 +365,8 @@ lemma invoke_tcb_silc_inv[FinalCaps_assms]:
   apply (strengthen use_no_cap_to_obj_asid_strg
          | clarsimp
          | simp only: conj_ac cong: conj_cong imp_cong
-         | wp checked_insert_pas_refined checked_cap_insert_silc_inv hoare_vcg_all_liftE_R
+         | wp case_option_wp_returnOk case_option_wp_return
+              checked_insert_pas_refined checked_cap_insert_silc_inv hoare_vcg_all_liftE_R
               hoare_vcg_all_lift hoare_vcg_const_imp_liftE_R
               cap_delete_silc_inv_not_transferable
               cap_delete_pas_refined' cap_delete_deletes
@@ -310,10 +390,12 @@ lemma invoke_tcb_silc_inv[FinalCaps_assms]:
          | wp (once) hoare_drop_imps
          | elim disjE; solves clarsimp)+
   (* also slow, ~30s *)
-  apply (intro impI conjI
-         | clarsimp simp: is_cap_simps is_cnode_or_valid_arch_def is_valid_vtable_root_def
-                          authorised_tcb_inv_def emptyable_def
-                   split: cap.splits option.splits)+
+  prefer 1
+  apply (clarsimp simp: is_cap_simps)
+  apply (clarsimp split: option.split_asm)
+  apply (clarsimp simp: is_cap_simps is_cnode_or_valid_arch_def is_valid_vtable_root_def
+                            authorised_tcb_inv_def emptyable_def
+                     split: cap.splits option.splits pt_type.splits arch_cap.splits)+
   done
 
 end
@@ -325,5 +407,55 @@ proof goal_cases
   case 1 show ?case
     by (unfold_locales; (fact FinalCaps_assms)?)
 qed
+
+
+context Arch begin global_naming AARCH64
+
+lemma handle_hypervisor_fault_silc_inv[FinalCaps_assms]:
+  "\<lbrace>silc_inv aag st and invs and pas_refined aag and is_subject aag o cur_thread and K (is_subject aag t)\<rbrace>
+   handle_hypervisor_fault t ex
+   \<lbrace>\<lambda>_. silc_inv aag st\<rbrace>"
+  apply (case_tac ex; clarsimp split del: if_split)
+  apply (wpsimp wp: handle_fault_silc_inv simp: valid_fault_def)
+  done
+
+lemma vppi_event_silc_inv:
+  "\<lbrace>silc_inv aag st and invs and pas_refined aag and (\<lambda>s. ct_active s \<longrightarrow> is_subject aag (cur_thread s))\<rbrace>
+   vppi_event irq
+   \<lbrace>\<lambda>_. silc_inv aag st\<rbrace>"
+  unfolding vppi_event_def
+  apply (wpsimp wp: gts_wp hoare_vcg_all_lift vcpu_update_trivial_invs maskInterrupt_invs
+                    hoare_vcg_imp_lift  | wps | wp dmo_wp)+
+  apply (clarsimp simp: valid_fault_def)
+  using ct_active_st_tcb_at_weaken runnable_eq by blast
+
+lemma vgic_maintenance_silc_inv:
+  "\<lbrace>silc_inv aag st and invs and pas_refined aag and (\<lambda>s. ct_active s \<longrightarrow> is_subject aag (cur_thread s))\<rbrace>
+   vgic_maintenance
+   \<lbrace>\<lambda>_. silc_inv aag st\<rbrace>"
+  unfolding vgic_maintenance_def
+  apply (wpsimp wp: gts_wp hoare_vcg_all_lift hoare_weak_lift_imp dmo_invs_lift
+              simp: crunch_simps valid_fault_def split_del: if_split
+         | wps | wp (once) hoare_drop_imps)+
+  using ct_active_st_tcb_at_weaken runnable_eq by blast
+
+lemma handle_reserved_irq_silc_inv[FinalCaps_assms]:
+  "\<lbrace>silc_inv aag st and invs and pas_refined aag and (\<lambda>s. ct_active s \<longrightarrow> is_subject aag (cur_thread s))\<rbrace>
+   handle_reserved_irq irq
+   \<lbrace>\<lambda>_. silc_inv aag st\<rbrace>"
+  unfolding handle_reserved_irq_def
+  by (cases "irq = irqVGICMaintenance"; wpsimp wp: vgic_maintenance_silc_inv vppi_event_silc_inv)
+
+end
+
+
+global_interpretation FinalCaps_3?: FinalCaps_3
+proof goal_cases
+  interpret Arch .
+  case 1 show ?case
+    apply (unfold_locales; (fact FinalCaps_assms)?)
+    sorry (* FIXME AARCH64 IF: weaken assumptions *)
+qed
+
 
 end
