proof/infoflow/AARCH64/ArchInterrupt_IF.thy
@@ -14,17 +14,25 @@ named_theorems Interrupt_IF_assms
 
 lemma arch_invoke_irq_handler_reads_respects[Interrupt_IF_assms, wp]:
   "reads_respects_f aag l (silc_inv aag st) (arch_invoke_irq_handler irq)"
-  apply (cases irq; wpsimp simp: plic_complete_claim_def)
-  apply (rule reads_respects_f[OF dmo_mol_reads_respects, where Q=\<top>, simplified])
-  apply wpsimp
+  apply (cases irq)
+    apply (wpsimp simp: plic_complete_claim_def deactivateInterrupt_def maskInterrupt_def)
+    apply (rule reads_respects_f[where P=\<top> and Q=\<top>, simplified])
+     apply (rule use_spec_ev)
+     apply (rule do_machine_op_spec_reads_respects)
+      apply (simp add: equiv_valid_def2)
+      apply (rule modify_ev2)
+      apply (fastforce simp: equiv_for_def)
+     apply (wp modify_wp | simp)+
   done
 
 lemma arch_invoke_irq_control_reads_respects[Interrupt_IF_assms]:
   "reads_respects aag (l :: 'a subject_label) (K (arch_authorised_irq_ctl_inv aag i))
                   (arch_invoke_irq_control i)"
   apply (cases i)
-  apply (simp add: setIRQTrigger_def)
-  apply (wp cap_insert_reads_respects set_irq_state_reads_respects dmo_mol_reads_respects | simp)+
+   apply (simp add: setIRQTrigger_def)
+   apply (wp cap_insert_reads_respects set_irq_state_reads_respects dmo_mol_reads_respects | simp)+
+   apply (clarsimp simp: arch_authorised_irq_ctl_inv_def)
+  apply (wpsimp wp: equiv_valid_guard_imp[OF cap_insert_reads_respects])
   apply (clarsimp simp: arch_authorised_irq_ctl_inv_def)
   done
 
@@ -33,14 +41,14 @@ lemma arch_invoke_irq_control_globals_equiv[Interrupt_IF_assms]:
    arch_invoke_irq_control ai
    \<lbrace>\<lambda>_. globals_equiv st\<rbrace>"
   apply (induct ai)
-  apply (simp add: setIRQTrigger_def)
-  apply (wpsimp wp: set_irq_state_globals_equiv set_irq_state_valid_global_objs
-                    cap_insert_globals_equiv'' dmo_mol_globals_equiv)
+   apply (simp add: setIRQTrigger_def)
+   apply (wpsimp wp: set_irq_state_globals_equiv set_irq_state_valid_global_objs
+                     cap_insert_globals_equiv'' dmo_mol_globals_equiv)+
   done
 
 lemma arch_invoke_irq_handler_globals_equiv[Interrupt_IF_assms, wp]:
   "arch_invoke_irq_handler irq \<lbrace>globals_equiv st\<rbrace>"
-  by (cases irq; wpsimp wp: dmo_no_mem_globals_equiv simp: plic_complete_claim_def)
+  by (cases irq; wpsimp wp: dmo_no_mem_globals_equiv simp: plic_complete_claim_def deactivateInterrupt_def)
 
 end
 
